@prefix afn:                  <http://jena.hpl.hp.com/ARQ/function#> .
@prefix arg:                  <http://spinrdf.org/arg#> .
@prefix causemod:             <http://nwcg.gov/model/fireCause#> .
@prefix corpus:               <http://topbraid.org/corpus#> .
@prefix crosswalk:            <http://topbraid.org/crosswalk#> .
@prefix crosswalk.spin:       <http://topbraid.org/crosswalk.spin#> .
@prefix crosswalkapp:         <http://topbraid.org/swa/crosswalkapp#> .
@prefix crosswalkprojects:    <http://teamwork.topbraidlive.org/crosswalkprojects#> .
@prefix dash:                 <http://datashapes.org/dash#> .
@prefix dc:                   <http://purl.org/dc/elements/1.1/> .
@prefix dct:                  <http://purl.org/dc/terms/> .
@prefix dcterms:              <http://purl.org/dc/terms/> .
@prefix debug-swa:            <http://debug.topbraidlive.org/1.0/swa/> .
@prefix edg:                  <http://edg.topbraid.solutions/model/> .
@prefix evnconstraints:       <http://topbraid.org/spin/evnconstraints#> .
@prefix fn:                   <http://www.w3.org/2005/xpath-functions#> .
@prefix governance:           <http://topbraid.org/teamworkgovernance.ui#> .
@prefix graphql:              <http://datashapes.org/graphql#> .
@prefix html:                 <http://uispin.org/html#> .
@prefix jfn:                  <java:org.apache.jena.sparql.function.library.> .
@prefix lib-importer:         <http://edg.topbraid.solutions/importer/lib#> .
@prefix list:                 <http://jena.apache.org/ARQ/list#> .
@prefix metadata:             <http://topbraid.org/metadata#> .
@prefix nlp:                  <http://topbraid.org/nlp#> .
@prefix ontologyprojects:     <http://teamwork.topbraidlive.org/ontologyprojects#> .
@prefix owl:                  <http://www.w3.org/2002/07/owl#> .
@prefix owlrl:                <http://topbraid.org/spin/owlrl#> .
@prefix pf:                   <http://jena.hpl.hp.com/ARQ/property#> .
@prefix rdf:                  <http://www.w3.org/1999/02/22-rdf-syntax-ns#> .
@prefix rdfs:                 <http://www.w3.org/2000/01/rdf-schema#> .
@prefix rdmprojects:          <http://rdm.topbraidlive.org/rdmprojects#> .
@prefix safindex:             <http://topbraid.org/safindex#> .
@prefix scheduler:            <http://topbraid.org/scheduler#> .
@prefix sh:                   <http://www.w3.org/ns/shacl#> .
@prefix sharepoint-termstore: <http://teamwork.topbraidlive.org/taxonomy/sharepoint-termstore#> .
@prefix skos:                 <http://www.w3.org/2004/02/skos/core#> .
@prefix skosshapes:           <http://topbraid.org/skos.shapes#> .
@prefix skosspin:             <http://topbraid.org/spin/skosspin#> .
@prefix skostemplate:         <http://topbraid.org/spin/skostemplates#> .
@prefix skosxl:               <http://www.w3.org/2008/05/skos-xl#> .
@prefix sm:                   <http://topbraid.org/sparqlmotion#> .
@prefix smf:                  <http://topbraid.org/sparqlmotionfunctions#> .
@prefix sml:                  <http://topbraid.org/sparqlmotionlib#> .
@prefix sp:                   <http://spinrdf.org/sp#> .
@prefix spif:                 <http://spinrdf.org/spif#> .
@prefix spin:                 <http://spinrdf.org/spin#> .
@prefix spinmap:              <http://spinrdf.org/spinmap#> .
@prefix spinmapl:             <http://topbraid.org/spin/spinmapl#> .
@prefix spl:                  <http://spinrdf.org/spl#> .
@prefix spr:                  <http://spinrdf.org/spr#> .
@prefix spra:                 <http://spinrdf.org/spra#> .
@prefix swa:                  <http://topbraid.org/swa#> .
@prefix swaclasses:           <http://topbraid.org/swaclasses#> .
@prefix swauml:               <http://topbraid.org/swauml#> .
@prefix swon:                 <http://uispin.org/swon#> .
@prefix tables:               <http://topbraid.org/tables#> .
@prefix tablesmap:            <http://topbraid.org/spin/tablesmap#> .
@prefix tasks:                <http://topbraid.org/tasks#> .
@prefix tbgeo:                <http://topbraid.org/tbgeo#> .
@prefix tbladmin:             <http://server.topbraidlive.org/system-applications/tbladmin#> .
@prefix teamwork:             <http://topbraid.org/teamwork#> .
@prefix teamworkconstraints:  <http://topbraid.org/teamworkconstraints#> .
@prefix teamworks3:           <http://teamwork.topbraidlive.org/ui/teamworks3#> .
@prefix teamworkupdate:       <http://teamworkAPI.topbraid.com/teamworkUpdate#> .
@prefix textindex:            <http://topbraid.org/textindex#> .
@prefix tops:                 <http://www.topbraid.org/tops#> .
@prefix tosh:                 <http://topbraid.org/tosh#> .
@prefix tosh.ui:              <http://topbraid.org/tosh.ui#> .
@prefix tracker:              <http://teamwork.topbraidlive.org/ui/tracker#> .
@prefix ui:                   <http://uispin.org/ui#> .
@prefix uix:                  <http://topbraidlive.org/uix#> .
@prefix xsd:                  <http://www.w3.org/2001/XMLSchema#> .

ontologyprojects:Ontology
        rdfs:subClassOf  teamwork:Vocabulary .

causemod:CLASS-ActivityGroup
        rdf:type         sh:NodeShape , owl:Class ;
        rdfs:comment     "Further refines information for prevention programs for targeted messaging. " ;
        rdfs:label       "Activity Group" ;
        rdfs:subClassOf  skos:Concept .

causemod:CLASS-GeneralCause
        rdf:type         sh:NodeShape , owl:Class ;
        rdfs:comment     "Agency or circumstance which started a fire or set the stage for its occurrence." ;
        rdfs:label       "General Cause" ;
        rdfs:subClassOf  skos:Concept .

teamwork:Vocabulary  rdfs:subClassOf  owl:Ontology .

causemod:CLASS-WildfireCause-label
        rdf:type         sh:PropertyShape ;
        dash:singleLine  true ;
        graphql:name     "labels" ;
        sh:name          "labels" ;
        sh:or            dash:StringOrLangString ;
        sh:path          rdfs:label .

<urn:x-evn-master:causemod>
        rdf:type              teamwork:Vocabulary , owl:Ontology , ontologyprojects:Ontology ;
        rdfs:comment          "A model describing fire cause within wildland fire. A representation of the Fire Cause Data Standard as established by NWCG." ;
        rdfs:label            "WF Schema - Wildland Fire Cause" ;
        edg:subjectArea       <urn:x-tb-governance:WF> ;
        metadata:status       metadata:UnderDevelopmentStatus ;
        swa:defaultNamespace  "http://nwcg.gov/model/fireCause#" ;
        owl:imports           <http://topbraid.org/teamworkconstraints> , <http://datashapes.org/graphql> , <http://topbraid.org/skos.shapes> .

causemod:CLASS-SpecificCauseDetail
        rdf:type         sh:NodeShape , owl:Class ;
        rdfs:comment     "More specific information about the cause or factors contributing to the ignition." ;
        rdfs:label       "Specific Cause Detail" ;
        rdfs:subClassOf  skos:Concept .

causemod:CLASS-CauseClassification
        rdf:type         sh:NodeShape , owl:Class ;
        rdfs:comment     "Broad classification of the reason the fire occurred." ;
        rdfs:label       "Cause Classification" ;
        rdfs:subClassOf  skos:Concept .

causemod:CLASS-SpecificCause
        rdf:type         sh:NodeShape , owl:Class ;
        rdfs:comment     "A further categorization of each General Cause to indicate more specifically the agency or circumstance which started a fire or set the stage for its occurrence." ;
        rdfs:label       "Specific Cause" ;
        rdfs:subClassOf  skos:Concept .

causemod:CLASS-WildfireCause
        rdf:type         sh:NodeShape , owl:Class ;
        rdfs:comment     "Identifying something that started a wildfire." ;
        rdfs:label       "Wildfire Cause" ;
        rdfs:subClassOf  owl:Thing ;
        sh:property      causemod:CLASS-WildfireCause-type , causemod:CLASS-WildfireCause-label .

causemod:CLASS-WildfireCause-type
        rdf:type      sh:PropertyShape ;
        graphql:name  "types" ;
        sh:class      rdfs:Class ;
        sh:name       "types" ;
        sh:path       rdf:type .

causemod:CLASS-Prohibited
        rdf:type         sh:NodeShape , owl:Class ;
        rdfs:comment     "Allows identification of an activity which is unlawful or otherwise prohibited (burn ban, unpermitted, etc.) by local authorities." ;
        rdfs:label       "Prohibited" ;
        rdfs:subClassOf  skos:Concept .

causemod:CLASS-AgeCategory
        rdf:type         sh:NodeShape , owl:Class ;
        rdfs:comment     "Discriminates between children (0-12), adolescents (13-17), and adults (18+)." ;
        rdfs:label       "Age Category" ;
        rdfs:subClassOf  skos:Concept .
